

React-tRace Core

Toby Ueno

November 11, 2025

Syntax:

Value $v ::= x \mid \text{true} \mid \text{false} \mid n \mid s \mid \lambda x : \tau. e \mid \mathcal{C} \mid \text{text } v \mid \text{tag}(v, \bar{v}, \bar{v})$
| $\text{attr}(v, v) \mid \text{onClick } v$
Expression $e ::= \text{return } v \mid \text{let } x = e \text{ in } e \mid v \mid v \oplus v \mid \text{if } v \text{ then } e \text{ else } e$
Top-level expr $\hat{e} ::= e \mid \text{let } (x, x_{\text{set}}) = \text{useState}^\ell(v) \text{ in } \hat{e} \mid \text{let } x = e \text{ in } \hat{e}$
Program $P ::= e \mid \text{let } x = e \text{ in } P \mid \text{let } \mathcal{C}(x : \tau) = \hat{e} \text{ in } P$
Type $\tau ::= \mathbf{1} \mid \text{bool} \mid \text{int} \mid \tau \xrightarrow{E} \tau \mid \text{view} \mid \text{component } \tau \mid \text{setter } \tau \mid \text{attr}$
Effect $E ::= \epsilon \mid \text{Mut}$

Internal representations:

Component declarations $\Delta ::= [\overline{\mathcal{C} \mapsto \tau}]$
Phase $\phi ::= \text{Init} \mid \text{Succ}$
Tree $t ::= \text{lit } v \mid \text{node}(id, v, \bar{v}, \bar{t}) \mid p$
Realized component $\pi ::= \{\text{spec} : \langle \mathcal{C}, v \rangle, \text{st} : [\overline{\ell \mapsto v}], \text{child} : t\}$
Tree memory $m ::= [\overline{p \mapsto \pi}]$
Component definitions $\mathcal{D} ::= [\overline{\mathcal{C} \mapsto x.\hat{e}}]$
Mode $\mu ::= \text{start}(P) \mid \text{idle} \mid \text{rerender}(m)$

Effect unification:

$$E_1 \circ E_2 = \begin{cases} \epsilon & E_1 = E_2 = \epsilon \\ \text{Mut} & \text{otherwise} \end{cases}$$

All typing judgments are relative to a fixed Δ , which can be determined prior to typechecking by iterating through all components in the program and noting their arguments' type annotations.

Value typing: $\Gamma \vdash_{\Delta} v : \tau$

$$\begin{array}{c}
\frac{x : \tau \in \Gamma}{\Gamma \vdash_{\Delta} x : \tau} \text{TVAl-VAR} \qquad \frac{}{\Gamma \vdash_{\Delta} () : \mathbf{1}} \text{TVAl-UNIT} \\
\\
\frac{}{\Gamma \vdash_{\Delta} \text{true} : \text{bool}} \text{TVAl-TRUE} \qquad \frac{}{\Gamma \vdash_{\Delta} \text{false} : \text{bool}} \text{TVAl-FALSE} \\
\\
\frac{}{\Gamma \vdash_{\Delta} n : \text{int}} \text{TVAl-INT} \qquad \frac{}{\Gamma \vdash_{\Delta} s : \text{string}} \text{TVAl-STR} \\
\\
\frac{\Gamma, x : \tau_1 \vdash_{\Delta} e : \tau_2 \mid E}{\Gamma \vdash_{\Delta} \lambda x : \tau_1. e : \tau_1 \xrightarrow{E} \tau_2} \text{TVAl-LAM} \qquad \frac{\mathcal{C} : \text{component } \tau \in \Delta}{\Gamma \vdash_{\Delta} \mathcal{C} : \text{component } \tau} \text{TVAl-COMP} \\
\\
\frac{\Gamma \vdash_{\Delta} v : \tau \quad \tau \in \{\text{bool}, \text{int}, \text{string}\}}{\Gamma \vdash_{\Delta} \text{text } v : \text{view}} \text{TVAl-TEXT} \\
\\
\frac{\Gamma \vdash_{\Delta} v : \text{string} \quad (\forall i) \Gamma \vdash_{\Delta} v_i : \text{attr} \quad (\forall j) \Gamma \vdash_{\Delta} v_j : \text{view}}{\Gamma \vdash_{\Delta} \text{tag}(v, \overline{v_i}, \overline{v_j}) : \text{view}} \text{TVAl-TAG} \\
\\
\frac{\Gamma \vdash_{\Delta} v_k : \text{string} \quad \Gamma \vdash_{\Delta} v_v : \text{string}}{\Gamma \vdash_{\Delta} \text{attr}(v_k, v_v) : \text{attr}} \text{TVAl-ATTR} \\
\\
\frac{\Gamma \vdash_{\Delta} v : \mathbf{1} \xrightarrow{E} \mathbf{1}}{\Gamma \vdash_{\Delta} \text{onClick } v : \text{attr}} \text{TVAl-ONCLICK}
\end{array}$$

Base expression typing: $\Gamma \vdash_{\Delta} e : x \mid E$

$$\begin{array}{c}
\frac{\Gamma \vdash_{\Delta} v : \tau}{\Gamma \vdash_{\Delta} \text{return } v : \tau \mid \epsilon} \text{TEXP-RET} \\
\\
\frac{\Gamma \vdash_{\Delta} e_1 : \tau_1 \mid E_1 \quad \Gamma, x : \tau_1 \vdash_{\Delta} e_2 : \tau_2 \mid E_2}{\Gamma \vdash_{\Delta} \text{let } x = e_1 \text{ in } e_2 : \tau_2 \mid E_1 \circ E_2} \text{TEXP-LET} \\
\\
\frac{\Gamma \vdash_{\Delta} v_1 : \tau_1 \xrightarrow{E} \tau_2 \quad \Gamma \vdash_{\Delta} v_2 : \tau_1}{\Gamma \vdash_{\Delta} v_1 \ v_2 : \tau_2 \mid E} \text{TEXP-APPFUN} \\
\\
\frac{\Gamma \vdash_{\Delta} v_1 : \text{component } \tau \quad \Gamma \vdash_{\Delta} v_2 : \tau}{\Gamma \vdash_{\Delta} v_1 \ v_2 : \text{view} \mid \epsilon} \text{TEXP-APPCOMP} \\
\\
\frac{\Gamma \vdash_{\Delta} v_1 : \text{setter } \tau \quad \Gamma \vdash_{\Delta} v_2 : \tau}{\Gamma \vdash_{\Delta} v_1 \ v_2 : \mathbf{1} \mid \text{Mut}} \text{TEXP-APPSET} \\
\\
\frac{\Gamma \vdash_{\Delta} v_1 : \text{int} \quad \Gamma \vdash_{\Delta} v_2 : \text{int} \quad \oplus : \mathbb{Z} \times \mathbb{Z} \rightarrow \mathbb{Z}}{\Gamma \vdash_{\Delta} v_1 \oplus v_2 : \text{int}} \text{TEXP-BOP} \\
\\
\frac{\Gamma \vdash_{\Delta} v : \text{bool} \quad \Gamma \vdash_{\Delta} e_1 : \tau \mid E_1 \quad \Gamma \vdash_{\Delta} e_2 : \tau \mid E_2}{\Gamma \vdash_{\Delta} \text{if } v \text{ then } e_1 \text{ else } e_2 : \tau \mid E_1 \circ E_2} \text{TEXP-IF}
\end{array}$$

Top-level expression typing: $\Gamma \Vdash_{\Delta} \hat{e} : \tau$

$$\frac{\Gamma \vdash_{\Delta} e : \tau \mid \epsilon}{\Gamma \Vdash_{\Delta} \hat{e} : \tau} \text{THAT-LIFT} \quad \frac{\Gamma \vdash_{\Delta} e : \tau_1 \mid \epsilon \quad \Gamma, x : \tau_1 \Vdash_{\Delta} \hat{e} : \tau_2}{\Gamma \Vdash_{\Delta} \text{let } x = e \text{ in } \hat{e} : \tau_2} \text{THAT-LET}$$

$$\frac{\Gamma \vdash_{\Delta} v : \tau_1 \quad \Gamma, x : \tau_1, x_{\text{set}} : \tau_1 \xrightarrow{\text{Set}} \mathbf{1} \Vdash_{\Delta} \hat{e} : \tau_2}{\Gamma \Vdash_{\Delta} \text{let } (x, x_{\text{set}}) = \text{useState}^{\ell}(v) \text{ in } \hat{e} : \tau_2} \text{THAT-STATE}$$

Program judgment: $\Gamma \vdash_{\Delta} P$

$$\frac{\Gamma \vdash_{\Delta} e : \tau \mid \epsilon \quad \Gamma, x : \tau \vdash_{\Delta} P}{\Gamma \vdash_{\Delta} \text{let } x = e \text{ in } P} \text{TPROG-LET}$$

$$\frac{\Gamma, x : \tau \Vdash_{\Delta} \hat{e} : \text{view} \quad \Gamma \vdash_{\Delta} P}{\Gamma \vdash_{\Delta} \text{let } \mathcal{C}(x : \tau) = \hat{e} \text{ in } P} \text{TPROG-COMP}$$

$$\frac{\Gamma \vdash_{\Delta} e : \text{view} \mid \epsilon}{\Gamma \vdash_{\Delta} \text{run } e} \text{TPROG-RUN}$$

Throughout the semantics, we use the notation $m' = m \mid x = v$ to concisely denote nested map/record updates. The above should be read as “ m' equals m with field x set to v ”. For instance, $m' = m \mid m[p].st[\ell] = v$ updates the state field of m at path p and location ℓ to value v and names the result m' .

Pure expression semantics: $m; e \mapsto e'; m'$

$\frac{m; e_1 \mapsto e'_1; m'}{m; \text{let } x = e_1 \text{ in } e_2 \mapsto \text{let } x = e'_1 \text{ in } e_2; m'} \text{E-LETPURE}$	
$m; \text{let } x = \text{return } v \text{ in } e \mapsto e[v/x]; m$	E-RET
$m; (\lambda x.e)v \mapsto e[v/x]; m$	E-APPFUN
$m; \mathcal{C} v \mapsto \langle \mathcal{C}, v \rangle; m$	E-APPComp
$m; \text{set@}_p^\ell v \mapsto (); m'$	E-APPSET
$(m' = m \mid m[p].st[\ell] = v)$	
$m; n_1 \oplus n_2 \mapsto \text{return } \llbracket n_1 \oplus n_2 \rrbracket; m$	E-BOP
$m; \text{if true then } e_1 \text{ else } e_2 \mapsto e_1; m$	E-IFTRUE
$m; \text{if false then } e_1 \text{ else } e_2 \mapsto e_2; m$	E-IFFALSE

Top-level expression semantics: $m; \hat{e} \mapsto_p^\phi \hat{e}'; m'$

$\frac{m; e \mapsto e'; m'}{m; e \mapsto_p^\phi e'; m'} \text{E-LIFT}$	
$\frac{m; e \mapsto e'; m'}{m; \text{let } x = e \text{ in } \hat{e} \mapsto_p^\phi \text{let } x = e' \text{ in } \hat{e}; m'} \text{E-LETTOP}$	
$m; \text{let } x = \text{return } v \text{ in } \hat{e} \mapsto_p^\phi \hat{e}[v/x]; m$	E-RETTOP
$m; \text{let } (x, x_{\text{set}}) = \text{useState}^\ell(v) \text{ in } \hat{e} \mapsto_p^{\text{Init}} \hat{e}[v/x, \text{set@}_p^\ell/x_{\text{set}}]; m'$	E-STINIT
$(m' = m \mid m[p].st[\ell] = v)$	
$m; \text{let } (x, x_{\text{set}}) = \text{useState}^\ell(v) \text{ in } \hat{e} \mapsto_p^{\text{Succ}} \hat{e}[v'/x, \text{set@}_p^\ell/x_{\text{set}}]; m$	E-STSUCC
$(v' = m[p].st[\ell])$	

Program expression semantics: $m; \mathcal{D}; P \Rightarrow P'; \mathcal{D}'; m'$

$$\frac{m; e \mapsto e'; m'}{m; \mathcal{D}; \text{run } e \Rightarrow \text{run } e'; \mathcal{D}; m'} \text{E-RUN}$$

$$\frac{m; e \mapsto e'; m'}{m; \mathcal{D}; \text{let } x = e \text{ in } P \Rightarrow \text{let } x = e' \text{ in } P; \mathcal{D}; m'} \text{E-LETPROG}$$

$$m; \mathcal{D}; \text{let } x = \text{return } v \text{ in } P \Rightarrow P[v/x]; \mathcal{D}; m \quad \text{E-RETPROG}$$

$$m; \mathcal{D}; \text{let } \mathcal{C}(x) = \hat{e} \text{ in } P \Rightarrow P; \mathcal{D}[\mathcal{C} \mapsto x.\hat{e}]; m \quad \text{E-COMPDEF}$$

Node initialization: $\mathcal{D}; m \vdash \text{init}(v) = \langle t, m' \rangle$

$$\frac{}{\mathcal{D}; m \vdash \text{init}(\text{text } v) = \langle \text{lit } v, m \rangle} \text{INIT-LIT}$$

$$\frac{id \text{ fresh} \quad (\forall j) \mathcal{D}; m_j \vdash \text{init}(v_j) = \langle t_j, m_{j+1} \rangle}{\mathcal{D}; m_0 \vdash \text{init}(\text{tag}(v, \overline{v_i}, \overline{v_{j=0}^{n-1}})) = \langle \text{node}(id, v, \overline{v_i}, \overline{t_j}), m_n \rangle} \text{INIT-NODE}$$

$$\frac{\begin{array}{c} m_0 \vdash p \text{ fresh} \quad \mathcal{D}[\mathcal{C}] = x.\hat{e} \\ m_0[p \mapsto \{\text{spec} : \langle \mathcal{C}, v \rangle, \text{st} : \emptyset, \text{child} : \emptyset\}]; \hat{e}[v/x] \xrightarrow{p}^{\text{Init}} \text{return } v'; m_1 \\ \mathcal{D}; m_1 \vdash \text{init}(v') = \langle t, m_2 \rangle \end{array}}{\mathcal{D}; m_0 \vdash \text{init}(\langle \mathcal{C}, v \rangle) = \langle p, m_2 \mid m_2[p].\text{child} = t \rangle} \text{INIT-COMP}$$

(Naïve) re-render: $\mathcal{D}; m_{\text{old}} \vdash \text{check}(m_{\text{new}}, t) = m$

$$\frac{}{\mathcal{D}; m_{\text{old}} \vdash \text{check}(m_{\text{new}}, \text{lit } v) = m_{\text{new}}} \text{CHECK-LIT}$$

$$\frac{(0 \leq j < n) \quad \mathcal{D}; m_{\text{old}} \vdash \text{check}(m_j, t_j) = \langle t'_j, m_{j+1} \rangle}{\mathcal{D}; m_{\text{old}} \vdash \text{check}(m_0, \text{node}(id, v, \overline{v_i}, \overline{t_j})) = m_n} \text{CHECK-NODE}$$

$$\frac{\begin{array}{c} m_{\text{old}}[p].\text{st} = m_{\text{new}}[p].\text{st} \\ \mathcal{D}; m_{\text{old}} \vdash \text{check}(m_{\text{new}}, m_{\text{old}}[p].\text{child}) = m \end{array}}{\mathcal{D}; m_{\text{old}} \vdash \text{check}(m_{\text{new}}, p) = m} \text{CHECK-PATHCONST}$$

$$\frac{\begin{array}{c} m_{\text{old}}[p].\text{st} \neq m_{\text{new}}[p].\text{st} \quad m'[p].\text{spec} = \langle \mathcal{C}, v \rangle \quad \mathcal{D}[\mathcal{C}] = x.\hat{e} \\ m_{\text{new}}; \hat{e}[v/x] \xrightarrow{p}^{\text{Succ}} \text{return } v'; m \\ \mathcal{D}; m \vdash \text{init}(v') = \langle t, m' \rangle \end{array}}{\mathcal{D}; m_{\text{old}} \vdash \text{check}(m_{\text{new}}, p) = \langle p, m' \mid m[p].\text{child} = t \rangle} \text{CHECK-PATHDIFF}$$

Event loop semantics: $\langle \mathcal{D}, m, t, \mu \rangle \hookrightarrow \langle \mathcal{D}', m', t, \mu' \rangle$

$$\frac{\cdot; \cdot; P \mapsto^* \text{run}(\text{return } v); \mathcal{D}; m \quad \mathcal{D}; m \vdash \text{init}(v) = \langle t, m' \rangle}{\langle \cdot, \cdot, \cdot, \text{start}(P) \rangle \hookrightarrow \langle \mathcal{D}, m', t, \text{idle} \rangle} \text{ LOOP-START}$$

$$\frac{\exists id \quad m \vdash \text{handlers}(t, id) = \bar{v}_i \quad (0 \leq i < n) \quad m_i; v_i () \mapsto^* \text{return } (); m_{i+1}}{\langle \mathcal{D}, m_0, t, \text{idle} \rangle \hookrightarrow \langle \mathcal{D}, m, t, \text{render}(m_n) \rangle} \text{ LOOP-EVENT}$$

$$\frac{D; m_{\text{old}} \vdash \text{check}(m_{\text{new}}, t) = m}{\langle \mathcal{D}, m_{\text{old}}, t, \text{render}(m_{\text{new}}) \rangle \hookrightarrow \langle \mathcal{D}, m, t, \text{idle} \rangle} \text{ LOOP-RERENDER}$$

Handler search: $m \vdash \text{handlers}(t, id) = \bar{v}$

$$\frac{}{m \vdash \text{handlers}(\text{lit } v, id) = \{\}} \text{ HANDLERS-LIT}$$

$$\frac{m \vdash \text{handlers}(m[p].\text{child}, id) = \bar{v}}{m \vdash \text{handlers}(p, id) = \bar{v}} \text{ HANDLERS-COMP}$$

$$\frac{}{m \vdash \text{handlers}(\text{node}(id, v, \bar{v}_i, \bar{v}_j), id) = \{v_h \mid \text{onClick } v_h \in \bar{v}_i\}} \text{ HANDLERS-TGT}$$

$$\frac{id \neq id' \quad (\forall j) \quad m \vdash \text{handlers}(v_j, id) = h_j}{m \vdash \text{handlers}(\text{node}(id', v, \bar{v}_i, \bar{v}_j), id) = \bigcup_{\forall j} h_j} \text{ HANDLERS-NODE}$$